ASM.thy
@@ -1,0 +1,45 @@
+theory ASM
+  imports "HOL-IMP.AExp"
+begin
+
+type_synonym val = int
+type_synonym vname = string
+datatype instr = LOADI val | LOAD vname | ADD
+type_synonym stack = "val list"
+type_synonym state = "vname \<Rightarrow> val"
+
+fun exec1 :: "instr \<Rightarrow> state \<Rightarrow> stack \<Rightarrow> stack option" where
+"exec1 (LOADI n) _ stk = Some(n # stk)" |
+"exec1 (LOAD x) s stk = Some(s(x) # stk)" |
+"exec1 ADD _ (j # i # stk) = Some((i + j) # stk)" |
+"exec1 ADD _ [v] = None" |
+"exec1 ADD _ [] = None" 
+
+fun exec :: "instr list \<Rightarrow> state \<Rightarrow> stack \<Rightarrow> stack option" where
+"exec [] _ stk = Some stk" |
+"exec (i#is) s stk = 
+  (case (exec1 i s stk) of
+    Some res \<Rightarrow> exec is s res |
+    None \<Rightarrow> None)"
+
+fun comp :: "aexp \<Rightarrow> instr list" where
+"comp (N n) = [LOADI n]" |
+"comp (V x) = [LOAD x]" |
+"comp (Plus e1 e2) = comp e1 @ comp e2 @ [ADD]" 
+
+fun aval :: "aexp \<Rightarrow> state \<Rightarrow> val" where
+  "aval (N n) s = n" |
+  "aval (V x) s = s x" |
+  "aval (Plus a1 a2) s = aval a1 s + aval a2 s"
+
+lemma exec_append: "exec is1 s stk = Some new_stk \<Longrightarrow> exec (is1 @ is2) s stk = exec is2 s new_stk"
+  apply(induction is1 arbitrary: stk)
+  apply(auto split: option.split)
+  done
+
+lemma "exec (comp a) s stk = Some ((aval a s) # stk)"
+  apply(induction a arbitrary: stk)
+  apply(auto simp add: exec_append)
+  done
+
+end
